Rename typing rules consistently
Also review derived rules, and fix some names of semantic typing lemmas.

theories/DSub/typing/typing_storeless.v
@@ -17,34 +17,34 @@ Reserved Notation "Γ s⊢ₜ[ g  ] e : T" (at level 74, e, T at next level).
 Reserved Notation "Γ s⊢ₜ[ g  ] T1 , i1 <: T2 , i2" (at level 74, T1, T2, i1, i2 at next level).
 
 Inductive typed Γ g : tm → ty → Prop :=
-| Appv_typed e1 v2 T1 T2:
+| iT_All_Ex e1 v2 T1 T2:
     Γ s⊢ₜ[ g ] e1: TAll T1 T2 →                        Γ s⊢ₜ[ g ] tv v2 : T1 →
     (*────────────────────────────────────────────────────────────*)
     Γ s⊢ₜ[ g ] tapp e1 (tv v2) : T2.|[v2/]
 (** Non-dependent application; allowed for any argument. *)
-| App_typed e1 e2 T1 T2:
+| iT_All_E e1 e2 T1 T2:
     Γ s⊢ₜ[ g ] e1: TAll T1 (shift T2) →      Γ s⊢ₜ[ g ] e2 : T1 →
     (*────────────────────────────────────────────────────────────*)
     Γ s⊢ₜ[ g ] tapp e1 e2 : T2
-| Lam_typed e T1 T2:
+| iT_All_I e T1 T2:
     (* T1 :: Γ s⊢ₜ[ g ] e : T2 → (* Would work, but allows the argument to occur in its own type. *) *)
     shift T1 :: Γ s⊢ₜ[ g ] e : T2 →
     (*─────────────────────────*)
     Γ s⊢ₜ[ g ] tv (vabs e) : TAll T1 T2
-| T_Nat_typed n:
+| iT_Nat_I n:
     Γ s⊢ₜ[ g ] tv (vnat n): TNat
 
 (** "General" rules *)
-| Var_typed x T :
+| iT_Var x T :
     (* After looking up in Γ, we must weaken T for the variables on top of x. *)
     Γ !! x = Some T →
     (*──────────────────────*)
     Γ s⊢ₜ[ g ] tv (var_vl x) : shiftN x T
-| Subs_typed e T1 T2 i :
+| iT_Sub e T1 T2 i :
     Γ s⊢ₜ[ g ] T1, 0 <: T2, i → Γ s⊢ₜ[ g ] e : T1 →
     (*───────────────────────────────*)
     Γ s⊢ₜ[ g ] iterate tskip i e : T2
-| Vty_abs_typed T L U σ s :
+| iT_Typ_Abs T L U σ s :
     T ~[ length Γ ] (g, (s, σ)) →
     Γ s⊢ₜ[ g ] T, 1 <: U, 1 →
     Γ s⊢ₜ[ g ] L, 1 <: T, 1 →
@@ -54,46 +54,46 @@ Inductive typed Γ g : tm → ty → Prop :=
 where "Γ s⊢ₜ[ g ] e : T " := (typed Γ g e T)
 with
 subtype Γ g : ty → nat → ty → nat → Prop :=
-| Refl_stp i T :
+| iSub_Refl i T :
     Γ s⊢ₜ[ g ] T, i <: T, i
 
-| Trans_stp i1 i2 i3 T1 T2 T3:
+| iSub_Trans i1 i2 i3 T1 T2 T3:
     Γ s⊢ₜ[ g ] T1, i1 <: T2, i2 → Γ s⊢ₜ[ g ] T2, i2 <: T3, i3 → Γ s⊢ₜ[ g ] T1, i1 <: T3, i3
 
 (* "Structural" rules about indexes *)
-| TSucc_stp T i:
+| iSub_Succ T i:
     Γ s⊢ₜ[ g ] T, i <: T, S i
-| TMono_stp T1 T2 i:
+| iSub_Mono T1 T2 i:
     Γ s⊢ₜ[ g ] T1, i <: T2, i →
     Γ s⊢ₜ[ g ] T1, S i <: T2, S i
 
 (* "Logical" connectives *)
-| Top_stp i T :
+| iSub_Top i T :
     Γ s⊢ₜ[ g ] T, i <: TTop, i
-| Bot_stp i T :
+| iBot_Sub i T :
     Γ s⊢ₜ[ g ] TBot, i <: T, i
 
 (* Type selections *)
-| SelU_stp L U v:
+| iSel_Sub L U v:
     Γ s⊢ₜ[ g ] tv v : TTMem L U →
     Γ s⊢ₜ[ g ] TSel v, 0 <: U, 1
 
-| LSel_stp L U v:
+| iSub_Sel L U v:
     Γ s⊢ₜ[ g ] tv v : TTMem L U →
     Γ s⊢ₜ[ g ] L, 1 <: TSel v, 0
 
 (* "Congruence" or "variance" rules for subtyping. Unneeded for "logical" types.
  "Cov" stands for covariance, "Con" for contravariance. *)
 (* Needed? Maybe drop later instead? *)
-(* | TLaterCov_stp T1 T2 i:
+(* | iLater_Sub_Later T1 T2 i:
     Γ s⊢ₜ[ g ] T1, S i <: T2, S i →
     Γ s⊢ₜ[ g ] TLater T1, i <: TLater T2, i *)
-| TAllConCov_stp T1 T2 U1 U2 i:
+| iAll_Sub_All T1 T2 U1 U2 i:
     (* "Tight" premises. *)
     Γ s⊢ₜ[ g ] T2, S i <: T1, S i →
     iterate TLater (S i) (shift T2) :: Γ s⊢ₜ[ g ] U1, S i <: U2, S i →
     Γ s⊢ₜ[ g ] TAll T1 U1, i <: TAll T2 U2, i
-| TTMemConCov_stp L1 L2 U1 U2 i:
+| iTyp_Sub_Typ L1 L2 U1 U2 i:
     Γ s⊢ₜ[ g ] L2, S i <: L1, S i →
     Γ s⊢ₜ[ g ] U1, S i <: U2, S i →
     Γ s⊢ₜ[ g ] TTMem L1 U1, i <: TTMem L2 U2, i
@@ -113,15 +113,15 @@ Abort. *)
 Lemma Vty_typed Γ g T L U σ s :
     T ~[ length Γ ] (g, (s, σ)) →
     Γ s⊢ₜ[ g ] tv (vstamp σ s) : TTMem T T.
-Proof. intros H. apply (Vty_abs_typed (T := T)); auto using Refl_stp. Qed.
+Proof. intros H. apply (iT_Typ_Abs (T := T)); auto using iSub_Refl. Qed.
 
 Scheme stamped_typed_mut_ind := Induction for typed Sort Prop
 with   stamped_subtype_mut_ind := Induction for subtype Sort Prop.
 Combined Scheme stamped_typing_mut_ind from stamped_typed_mut_ind, stamped_subtype_mut_ind.
 
 Hint Constructors subtype typed : core.
-Remove Hints Trans_stp : core.
-Hint Extern 10 => try_once Trans_stp : core.
+Remove Hints iSub_Trans : core.
+Hint Extern 10 => try_once iSub_Trans : core.
 
 Lemma stamped_typing_mono_mut Γ g:
   (∀ e T, Γ s⊢ₜ[ g ] e : T → ∀ g' (Hle: g ⊆ g'), Γ s⊢ₜ[ g' ] e : T) ∧
