theories/Dot/typing/typing_storeless.v
@@ -28,12 +28,12 @@ Judgments for typing, subtyping, path and definition typing.
 Inductive typed Γ g : tm → ty → Prop :=
 (** First, elimination forms *)
 (** Dependent application; only allowed if the argument is a value . *)
-| Appv_typed e1 v2 T1 T2:
+| iT_All_Ex e1 v2 T1 T2:
     Γ v⊢ₜ[ g ] e1: TAll T1 T2 →                        Γ v⊢ₜ[ g ] tv v2 : T1 →
     (*────────────────────────────────────────────────────────────*)
     Γ v⊢ₜ[ g ] tapp e1 (tv v2) : T2.|[v2/]
 
-| App_path_typed p2 e1 T1 T2 T2':
+| iT_All_Ex_p p2 e1 T1 T2 T2':
     T2 .Tp[ p2 /]~ T2' →
     is_stamped_ty (length Γ) g T2' →
     Γ v⊢ₜ[ g ] e1: TAll T1 T2 →
@@ -41,64 +41,64 @@ Inductive typed Γ g : tm → ty → Prop :=
     (*────────────────────────────────────────────────────────────*)
     Γ v⊢ₜ[ g ] tapp e1 (path2tm p2) : T2'
 (** Non-dependent application; allowed for any argument. *)
-| App_typed e1 e2 T1 T2:
+| iT_All_E e1 e2 T1 T2:
     Γ v⊢ₜ[ g ] e1: TAll T1 (shift T2) →      Γ v⊢ₜ[ g ] e2 : T1 →
     (*────────────────────────────────────────────────────────────*)
     Γ v⊢ₜ[ g ] tapp e1 e2 : T2
-| Proj_typed e T l:
+| iT_Obj_E e T l:
     Γ v⊢ₜ[ g ] e : TVMem l T →
     (*─────────────────────────*)
     Γ v⊢ₜ[ g ] tproj e l : T
-| TMuE_typed v T:
+| iT_Mu_E v T:
     Γ v⊢ₜ[ g ] tv v: TMu T →
     (*──────────────────────*)
     Γ v⊢ₜ[ g ] tv v: T.|[v/]
 (** Introduction forms *)
-| Lam_typed_strong e T1 T2 Γ':
+| iT_All_I_Strong e T1 T2 Γ':
     ⊢G Γ <:* TLater <$> Γ' →
     is_stamped_ty (length Γ) g T1 →
     (* T1 :: Γ' v⊢ₜ[ g ] e : T2 → (* Would work, but allows the argument to occur in its own type. *) *)
     shift T1 :: Γ' v⊢ₜ[ g ] e : T2 →
     (*─────────────────────────*)
     Γ v⊢ₜ[ g ] tv (vabs e) : TAll T1 T2
-| VObj_typed ds T:
+| iT_Obj_I ds T:
     Γ |L T v⊢ds[ g ] ds: T →
     is_stamped_ty (S (length Γ)) g T →
     (*──────────────────────*)
     Γ v⊢ₜ[ g ] tv (vobj ds): TMu T
-| TMuI_typed v T:
+| iT_Mu_I v T:
     Γ v⊢ₜ[ g ] tv v: T.|[v/] →
     (*──────────────────────*)
     Γ v⊢ₜ[ g ] tv v: TMu T
 
 (** "General" rules *)
-| Var_typed x T :
+| iT_Var x T :
     (* After looking up in Γ, we must weaken T for the variables on top of x. *)
     Γ !! x = Some T →
     (*──────────────────────*)
     Γ v⊢ₜ[ g ] tv (var_vl x) : shiftN x T
-| Subs_typed e T1 T2 i :
+| iT_Sub e T1 T2 i :
     Γ v⊢ₜ[ g ] T1, 0 <: T2, i → Γ v⊢ₜ[ g ] e : T1 →
     (*───────────────────────────────*)
     Γ v⊢ₜ[ g ] iterate tskip i e : T2
-| Path_typed p T :
+| iT_Path p T :
     Γ v⊢ₚ[ g ] p : T, 0 →
     (*───────────────────────────────*)
     Γ v⊢ₜ[ g ] path2tm p : T
 
 (** Primitives. *)
-| T_Nat_typed n:
+| iT_Nat_I n:
     Γ v⊢ₜ[ g ] tv (vnat n): TNat
-| T_Bool_typed b:
+| iT_Bool_I b:
     Γ v⊢ₜ[ g ] tv (vbool b): TBool
-| T_Un_typed u e1 B1 Br (Hu : un_op_syntype u B1 Br) :
+| iT_Un u e1 B1 Br (Hu : un_op_syntype u B1 Br) :
     Γ v⊢ₜ[ g ] e1 : TPrim B1 →
     Γ v⊢ₜ[ g ] tun u e1 : TPrim Br
-| T_Bin_typed b e1 e2 B1 B2 Br (Hu : bin_op_syntype b B1 B2 Br) :
+| iT_Bin b e1 e2 B1 B2 Br (Hu : bin_op_syntype b B1 B2 Br) :
     Γ v⊢ₜ[ g ] e1 : TPrim B1 →
     Γ v⊢ₜ[ g ] e2 : TPrim B2 →
     Γ v⊢ₜ[ g ] tbin b e1 e2 : TPrim Br
-| T_If_typed e e1 e2 T :
+| iT_If e e1 e2 T :
     Γ v⊢ₜ[ g ] e: TBool →
     Γ v⊢ₜ[ g ] e1 : T →
     Γ v⊢ₜ[ g ] e2 : T →
@@ -110,9 +110,9 @@ Inductive typed Γ g : tm → ty → Prop :=
     Γ v⊢ₜ[ g ] e : T *)
 where "Γ v⊢ₜ[ g ] e : T " := (typed Γ g e T)
 with dms_typed Γ g : dms → ty → Prop :=
-| dnil_typed : Γ v⊢ds[ g ] [] : TTop
+| iD_Nil : Γ v⊢ds[ g ] [] : TTop
 (* This demands definitions and members to be defined in aligned lists. *)
-| dcons_typed l d ds T1 T2:
+| iD_Cons l d ds T1 T2:
     Γ v⊢[ g ]{ l := d } : T1 →
     Γ v⊢ds[ g ] ds : T2 →
     dms_hasnt ds l →
@@ -120,66 +120,66 @@ with dms_typed Γ g : dms → ty → Prop :=
     Γ v⊢ds[ g ] (l, d) :: ds : TAnd T1 T2
 where "Γ v⊢ds[ g ] ds : T" := (dms_typed Γ g ds T)
 with dm_typed Γ g : label → dm → ty → Prop :=
-| dty_typed T l L U s σ:
+| iD_Typ_Abs T l L U s σ:
     T ~[ length Γ ] (g, (s, σ)) →
     is_stamped_σ (length Γ) g σ →
     Γ v⊢ₜ[ g ] TLater L, 0 <: TLater T, 0 →
     Γ v⊢ₜ[ g ] TLater T, 0 <: TLater U, 0 →
     Γ v⊢[ g ]{ l := dtysem σ s } : TTMem l L U
-| dpt_pv_typed l v T:
+| iD_Val l v T:
     Γ v⊢ₜ[ g ] tv v : T →
     Γ v⊢[ g ]{ l := dpt (pv v) } : TVMem l T
-| dpath_typed l p T:
+| iD_Path l p T:
     Γ v⊢ₚ[ g ] p : T, 0 →
     Γ v⊢[ g ]{ l := dpt p } : TVMem l T
-| dnew_typed l T ds:
+| iD_Val_New l T ds:
     TAnd (TLater T) (TSing (pself (pv (ids 1)) l)) :: Γ v⊢ds[ g ] ds : T →
     is_stamped_ty (S (length Γ)) g T →
     Γ v⊢[ g ]{ l := dpt (pv (vobj ds)) } : TVMem l (TMu T)
-| dpt_sub_typed T1 T2 p l:
+| iD_Path_Sub T1 T2 p l:
     Γ v⊢ₜ[ g ] T1, 0 <: T2, 0 →
     Γ v⊢[ g ]{ l := dpt p } : TVMem l T1 →
     Γ v⊢[ g ]{ l := dpt p } : TVMem l T2
 where "Γ v⊢[ g ]{ l := d  } : T" := (dm_typed Γ g l d T)
 with path_typed Γ g : path → ty → nat → Prop :=
-| pv_typed v T:
+| iP_Val v T:
     Γ v⊢ₜ[ g ] tv v : T →
     Γ v⊢ₚ[ g ] pv v : T, 0
 (* Mnemonic: Path from SELecting a Field *)
-| pself_typed p T i l:
+| iP_Fld_E p T i l:
     Γ v⊢ₚ[ g ] p : TVMem l T, i →
     Γ v⊢ₚ[ g ] pself p l : T, i
-| p_subs_typed p T1 T2 i j :
+| iP_Sub p T1 T2 i j :
     Γ v⊢ₜ[ g ] T1, i <: T2, i + j →
     Γ v⊢ₚ[ g ] p : T1, i →
     (*───────────────────────────────*)
     Γ v⊢ₚ[ g ] p : T2, i + j
-| p_mu_i_typed p T {T' i} :
+| iP_Mu_I p T {T' i} :
     T .Tp[ p /]~ T' →
     is_stamped_ty (S (length Γ)) g T →
     Γ v⊢ₚ[ g ] p : T', i →
     Γ v⊢ₚ[ g ] p : TMu T, i
-| p_mu_e_typed p T {T' i} :
+| iP_Mu_E p T {T' i} :
     T .Tp[ p /]~ T' →
     is_stamped_ty (length Γ) g T' →
     Γ v⊢ₚ[ g ] p : TMu T, i →
     Γ v⊢ₚ[ g ] p : T', i
-| pself_inv_typed p T i l:
+| iP_Fld_I p T i l:
     Γ v⊢ₚ[ g ] pself p l : T, i →
     (*─────────────────────────*)
     Γ v⊢ₚ[ g ] p : TVMem l T, i
-| psingleton_refl_typed T p i :
+| iP_Sngl_Refl T p i :
     Γ v⊢ₚ[ g ] p : T, i →
     Γ v⊢ₚ[ g ] p : TSing p, i
-| psingleton_inv_typed p q i:
+| iP_Sngl_Inv p q i:
     Γ v⊢ₚ[ g ] p : TSing q, i →
     is_stamped_path (length Γ) g q →
     Γ v⊢ₚ[ g ] q : TTop, i
-| psingleton_trans p q T i:
+| iP_Sngl_Trans p q T i:
     Γ v⊢ₚ[ g ] p : TSing q, i →
     Γ v⊢ₚ[ g ] q : T, i →
     Γ v⊢ₚ[ g ] p : T, i
-| psingleton_elim T p q l i:
+| iP_Sngl_E T p q l i:
     Γ v⊢ₚ[ g ] p : TSing q, i →
     Γ v⊢ₚ[ g ] pself q l : T, i →
     Γ v⊢ₚ[ g ] pself p l : TSing (pself q l), i
@@ -191,109 +191,109 @@ with path_typed Γ g : path → ty → nat → Prop :=
 where "Γ v⊢ₚ[ g ] p : T , i" := (path_typed Γ g p T i)
 (* Γ v⊢ₜ[ g ] T1, i1 <: T2, i2 means that TLater^i1 T1 <: TLater^i2 T2. *)
 with subtype Γ g : ty → nat → ty → nat → Prop :=
-| Refl_stp i T :
+| iSub_Refl i T :
     is_stamped_ty (length Γ) g T →
     Γ v⊢ₜ[ g ] T, i <: T, i
-| Trans_stp i2 T2 {i1 i3 T1 T3}:
+| iSub_Trans i2 T2 {i1 i3 T1 T3}:
     Γ v⊢ₜ[ g ] T1, i1 <: T2, i2 →
     Γ v⊢ₜ[ g ] T2, i2 <: T3, i3 →
     Γ v⊢ₜ[ g ] T1, i1 <: T3, i3
-| TLaterL_stp i T:
+| iLater_Sub i T:
     is_stamped_ty (length Γ) g T →
     Γ v⊢ₜ[ g ] TLater T, i <: T, S i
-| TLaterR_stp i T:
+| iSub_Later i T:
     is_stamped_ty (length Γ) g T →
     Γ v⊢ₜ[ g ] T, S i <: TLater T, i
 
 (* "Structural" rule about indexes *)
-| TAddLater_stp T i:
+| iSub_Add_Later T i:
     is_stamped_ty (length Γ) g T →
     Γ v⊢ₜ[ g ] T, i <: TLater T, i
 
 (* "Logical" connectives *)
-| Top_stp i T :
+| iSub_Top i T :
     is_stamped_ty (length Γ) g T →
     Γ v⊢ₜ[ g ] T, i <: TTop, i
-| Bot_stp i T :
+| iBot_Sub i T :
     is_stamped_ty (length Γ) g T →
     Γ v⊢ₜ[ g ] TBot, i <: T, i
-| TAnd1_stp T1 T2 i:
+| iAnd1_Sub T1 T2 i:
     is_stamped_ty (length Γ) g T1 →
     is_stamped_ty (length Γ) g T2 →
     Γ v⊢ₜ[ g ] TAnd T1 T2, i <: T1, i
-| TAnd2_stp T1 T2 i:
+| iAnd2_Sub T1 T2 i:
     is_stamped_ty (length Γ) g T1 →
     is_stamped_ty (length Γ) g T2 →
     Γ v⊢ₜ[ g ] TAnd T1 T2, i <: T2, i
-| TAnd_stp T U1 U2 i j:
+| iSub_And T U1 U2 i j:
     Γ v⊢ₜ[ g ] T, i <: U1, j →
     Γ v⊢ₜ[ g ] T, i <: U2, j →
     Γ v⊢ₜ[ g ] T, i <: TAnd U1 U2, j
-| TOr1_stp T1 T2 i:
+| iSub_Or1 T1 T2 i:
     is_stamped_ty (length Γ) g T1 →
     is_stamped_ty (length Γ) g T2 →
     Γ v⊢ₜ[ g ] T1, i <: TOr T1 T2, i
-| TOr2_stp T1 T2 i:
+| iSub_Or2 T1 T2 i:
     is_stamped_ty (length Γ) g T1 →
     is_stamped_ty (length Γ) g T2 →
     Γ v⊢ₜ[ g ] T2, i <: TOr T1 T2, i
-| TOr_stp T1 T2 U i j:
+| iOr_Sub T1 T2 U i j:
     Γ v⊢ₜ[ g ] T1, i <: U, j →
     Γ v⊢ₜ[ g ] T2, i <: U, j →
     Γ v⊢ₜ[ g ] TOr T1 T2, i <: U, j
 
 (* Type selections *)
-| SelU_stp p L {l U i}:
+| iSel_Sub p L {l U i}:
     Γ v⊢ₚ[ g ] p : TTMem l L U, i →
     Γ v⊢ₜ[ g ] TSel p l, i <: TLater U, i
-| LSel_stp p U {l L i}:
+| iSub_Sel p U {l L i}:
     Γ v⊢ₚ[ g ] p : TTMem l L U, i →
     Γ v⊢ₜ[ g ] TLater L, i <: TSel p l, i
-| PSub_singleton_stp p q {i T1 T2}:
+| iSngl_pq_Sub p q {i T1 T2}:
     T1 ~Tp[ p := q ]* T2 →
     is_stamped_ty (length Γ) g T1 →
     is_stamped_ty (length Γ) g T2 →
     Γ v⊢ₚ[ g ] p : TSing q, i →
     Γ v⊢ₜ[ g ] T1, i <: T2, i
-| PSym_singleton_stp T {p q i}:
+| iSngl_Sub_Sym T {p q i}:
     Γ v⊢ₚ[ g ] p : T, i →
     Γ v⊢ₜ[ g ] TSing p, i <: TSing q, i →
     Γ v⊢ₜ[ g ] TSing q, i <: TSing p, i
-| PSelf_singleton_stp {p T i} :
+| iSngl_Sub_Self {p T i} :
     Γ v⊢ₚ[ g ] p : T, i →
     Γ v⊢ₜ[ g ] TSing p, i <: T, i
 
 (* TODO: figure out if the drugs I had when I wrote these rules were good or bad. *)
-(* | SelU_stp l L U p i j: *)
+(* | iSel_Sub l L U p i j: *)
 (*     Γ v⊢ₚ[ g ] p : TTMem l L U, i → *)
 (*     Γ v⊢ₜ[ g ] TSel p l, j <: U, S (i + j) *)
-(* | LSel_stp l L U p i j: *)
+(* | iSub_Sel l L U p i j: *)
 (*     Γ v⊢ₚ[ g ] p : TTMem l L U, i → *)
 (*     Γ v⊢ₜ[ g ] L, S (i + j) <: TSel p l, j *)
 
 (* Subtyping for recursive types. Congruence, and opening in both directions. *)
-| Mu_stp_mu T1 T2 i j:
+| iMu_Sub_Mu T1 T2 i j:
     (iterate TLater i T1 :: Γ) v⊢ₜ[ g ] T1, i <: T2, j →
     is_stamped_ty (S (length Γ)) g T1 →
     Γ v⊢ₜ[ g ] TMu T1, i <: TMu T2, j
-| Mu_stp T i:
+| iMu_Sub T i:
     is_stamped_ty (length Γ) g T →
     Γ v⊢ₜ[ g ] TMu (shift T), i <: T, i
-| Stp_mu T i:
+| iSub_Mu T i:
     is_stamped_ty (length Γ) g T →
     Γ v⊢ₜ[ g ] T, i <: TMu (shift T), i
 
 (* "Congruence" or "variance" rules for subtyping. Unneeded for "logical" types.
  "Cov" stands for covariance, "Con" for contravariance. *)
-| TAllConCov_stp T1 T2 U1 U2 i:
+| iAll_Sub_All T1 T2 U1 U2 i:
     Γ v⊢ₜ[ g ] TLater T2, i <: TLater T1, i →
     iterate TLater (S i) (shift T2) :: Γ v⊢ₜ[ g ] TLater U1, i <: TLater U2, i →
     is_stamped_ty (length Γ) g T2 →
     Γ v⊢ₜ[ g ] TAll T1 U1, i <: TAll T2 U2, i
-| TVMemCov_stp T1 T2 i l:
+| iFld_Sub_Fld T1 T2 i l:
     Γ v⊢ₜ[ g ] T1, i <: T2, i →
     Γ v⊢ₜ[ g ] TVMem l T1, i <: TVMem l T2, i
-| TTMemConCov_stp L1 L2 U1 U2 i l:
+| iTyp_Sub_Typ L1 L2 U1 U2 i l:
     Γ v⊢ₜ[ g ] TLater L2, i <: TLater L1, i →
     Γ v⊢ₜ[ g ] TLater U1, i <: TLater U2, i →
     Γ v⊢ₜ[ g ] TTMem l L1 U1, i <: TTMem l L2 U2, i
@@ -302,21 +302,21 @@ with subtype Γ g : ty → nat → ty → nat → Prop :=
     F[A ∧ B] <: F[A] ∧ F[B] is provable by covariance.
     Let's prove F[A] ∧ F[B] <: F[A ∧ B] in the model.
     *)
-| TAllDistr_stp T U1 U2 i:
+| iAnd_All_Sub_Distr T U1 U2 i:
     is_stamped_ty (length Γ) g T →
     is_stamped_ty (S (length Γ)) g U1 →
     is_stamped_ty (S (length Γ)) g U2 →
     Γ v⊢ₜ[ g ] TAnd (TAll T U1) (TAll T U2), i <: TAll T (TAnd U1 U2), i
-| TVMemDistr_stp l T1 T2 i:
+| iAnd_Fld_Sub_Distr l T1 T2 i:
     is_stamped_ty (length Γ) g T1 →
     is_stamped_ty (length Γ) g T2 →
     Γ v⊢ₜ[ g ] TAnd (TVMem l T1) (TVMem l T2), i <: TVMem l (TAnd T1 T2), i
-| TTMemDistr_stp l L U1 U2 i:
+| iAnd_Typ_Sub_Distr l L U1 U2 i:
     is_stamped_ty (length Γ) g L →
     is_stamped_ty (length Γ) g U1 →
     is_stamped_ty (length Γ) g U2 →
     Γ v⊢ₜ[ g ] TAnd (TTMem l L U1) (TTMem l L U2), i <: TTMem l L (TAnd U1 U2), i
-| DistrAndOr1_stp {S T U i}:
+| iAnd_Or_Sub_Distr {S T U i}:
     is_stamped_ty (length Γ) g S →
     is_stamped_ty (length Γ) g T →
     is_stamped_ty (length Γ) g U →
@@ -339,7 +339,7 @@ with subtype Γ g : ty → nat → ty → nat → Prop :=
 where "Γ v⊢ₜ[ g ] T1 , i1 <: T2 , i2" := (subtype Γ g T1 i1 T2 i2).
 
 (* Make [T] first argument: Hide [Γ] and [g] for e.g. typing examples. *)
-Global Arguments dty_typed {Γ g} T _ _ _ _ _ _ _ _ _ : assert.
+Global Arguments iD_Typ_Abs {Γ g} T _ _ _ _ _ _ _ _ _ : assert.
 
 Scheme exp_stamped_typed_mut_ind := Induction for typed Sort Prop
 with   exp_stamped_dms_typed_mut_ind := Induction for dms_typed Sort Prop
@@ -359,20 +359,20 @@ with   stamped_subtype_mut_ind := Induction for subtype Sort Prop.
 Combined Scheme stamped_typing_mut_ind from stamped_typed_mut_ind, stamped_dms_typed_mut_ind,
   stamped_dm_typed_mut_ind, stamped_path_typed_mut_ind, stamped_subtype_mut_ind.
 
-Lemma Lam_typed Γ e T1 T2 g:
+Lemma iT_All_I Γ e T1 T2 g:
   is_stamped_ty (length Γ) g T1 →
   shift T1 :: Γ v⊢ₜ[ g ] e : T2 →
   (*─────────────────────────*)
   Γ v⊢ₜ[ g ] tv (vabs e) : TAll T1 T2.
-Proof. apply Lam_typed_strong. ietp_weaken_ctx. Qed.
+Proof. apply iT_All_I_Strong. ietp_weaken_ctx. Qed.
 
-Lemma Lam_typed_strip1 Γ e V T1 T2 g:
+Lemma iT_All_I_strip1 Γ e V T1 T2 g:
   is_stamped_ty (S (length Γ)) g T1 →
   shift T1 :: V :: Γ v⊢ₜ[ g ] e : T2 →
   (*─────────────────────────*)
   Γ |L V v⊢ₜ[ g ] tv (vabs e) : TAll T1 T2.
 Proof.
-  intros. apply (Lam_typed_strong (Γ' := (V :: Γ))) => //.
+  intros. apply (iT_All_I_Strong (Γ' := (V :: Γ))) => //.
   rewrite /defCtxCons/=; ietp_weaken_ctx.
 Qed.
 
@@ -380,18 +380,18 @@ Lemma dvabs_typed' Γ V T1 T2 e l g:
   is_stamped_ty (S (length Γ)) g T1 →
   shift T1 :: V :: Γ v⊢ₜ[ g ] e : T2 →
   Γ |L V v⊢[ g ]{ l := dpt (pv (vabs e)) } : TVMem l (TAll T1 T2).
-Proof. by intros; apply dpt_pv_typed, Lam_typed_strip1. Qed.
+Proof. by intros; apply iD_Val, iT_All_I_strip1. Qed.
 
 Lemma pv_dlater {Γ p T i g} :
   is_stamped_ty (length Γ) g T →
   Γ v⊢ₚ[ g ] p : TLater T, i →
   Γ v⊢ₚ[ g ] p : T, S i.
 Proof.
-  intros Hu Hp; apply p_subs_typed with (j := 1) (T1 := TLater T) (T2 := T) in Hp;
+  intros Hu Hp; apply iP_Sub with (j := 1) (T1 := TLater T) (T2 := T) in Hp;
     move: Hp; rewrite (plusnS i 0) (plusnO i); intros; by [|constructor].
 Qed.
 
-Ltac ettrans := eapply Trans_stp.
+Ltac ettrans := eapply iSub_Trans.
 
 (* Lemma Delay_stp {Γ g T1 T2 i j} :
   Γ v⊢ₜ[ g ] T1, i <: T2, j → TLater <$> Γ v⊢ₜ[ g ] TLater T1, i <: TLater T2, j.
@@ -402,15 +402,15 @@ Lemma TLater_Mono_stp {Γ g T1 T2 i j} :
   Γ v⊢ₜ[ g ] TLater T1, i <: TLater T2, j.
 Proof. intros Hs; eapply Undelay_stp, Delay_stp, Hs; ietp_weaken_ctx. Qed. *)
 
-(* Lemma TMono_stp {Γ T1 T2 i j g} :
+(* Lemma iSub_Mono {Γ T1 T2 i j g} :
   Γ v⊢ₜ[ g ] T1, i <: T2, j →
   is_stamped_ty (length Γ) g T1 →
   is_stamped_ty (length Γ) g T2 →
   Γ v⊢ₜ[ g ] T1, S i <: T2, S j.
 Proof.
   intros.
-  ettrans; first exact: TLaterR_stp.
-  ettrans; last exact: TLaterL_stp.
+  ettrans; first exact: iSub_Later.
+  ettrans; last exact: iLater_Sub.
   exact: TLater_Mono_stp.
 Qed. *)
 
@@ -420,8 +420,8 @@ Lemma Sub_later_shift {Γ T1 T2 i j g}
   (Hsub: Γ v⊢ₜ[ g ] T1, S i <: T2, S j):
   Γ v⊢ₜ[ g ] TLater T1, i <: TLater T2, j.
 Proof.
-  ettrans; first exact: TLaterL_stp.
-  by eapply Trans_stp, TLaterR_stp.
+  ettrans; first exact: iLater_Sub.
+  by eapply iSub_Trans, iSub_Later.
 Qed.
 
 Lemma Sub_later_shift_inv {Γ T1 T2 i j g}
@@ -430,8 +430,8 @@ Lemma Sub_later_shift_inv {Γ T1 T2 i j g}
   (Hsub: Γ v⊢ₜ[ g ] TLater T1, i <: TLater T2, j):
   Γ v⊢ₜ[ g ] T1, S i <: T2, S j.
 Proof.
-  ettrans; first exact: TLaterR_stp.
-  by eapply Trans_stp, TLaterL_stp.
+  ettrans; first exact: iSub_Later.
+  by eapply iSub_Trans, iLater_Sub.
 Qed.
 
 Ltac typconstructor_check :=
@@ -441,7 +441,7 @@ Ltac typconstructor_check :=
   end.
 Ltac typconstructor :=
   match goal with
-  | |- typed _ _ _ _ => first [apply Lam_typed_strip1 | apply Lam_typed | constructor]
+  | |- typed _ _ _ _ => first [apply iT_All_I_strip1 | apply iT_All_I | constructor]
   | |- dms_typed _ _ _ _ => constructor
   | |- dm_typed _ _ _ _ _ => first [apply dvabs_typed' | constructor]
   | |- path_typed _ _ _ _ _ => first [apply pv_dlater | constructor]
