theories/Dot/typing/typing_unstamped.v
@@ -26,7 +26,7 @@ Judgments for typing, subtyping, path and definition typing.
 Inductive typed Γ : tm → ty → Prop :=
 (** First, elimination forms *)
 (** Dependent application; only allowed if the argument is a path. *)
-| App_path_typed p2 e1 T1 T2:
+| iT_All_Ex_p p2 e1 T1 T2:
     is_unstamped_ty' (S (length Γ)) T2 →
     is_unstamped_path' (length Γ) p2 →
     (* T2 .Tp[ p2 /]~ T2' → *)
@@ -35,65 +35,65 @@ Inductive typed Γ : tm → ty → Prop :=
     (*────────────────────────────────────────────────────────────*)
     Γ u⊢ₜ tapp e1 (path2tm p2) : T2 .Tp[ p2 /]
 (** Non-dependent application; allowed for any argument. *)
-| App_typed e1 e2 T1 T2:
+| iT_All_E e1 e2 T1 T2:
     Γ u⊢ₜ e1: TAll T1 (shift T2) →      Γ u⊢ₜ e2 : T1 →
     (*────────────────────────────────────────────────────────────*)
     Γ u⊢ₜ tapp e1 e2 : T2
-| Proj_typed e T l:
+| iT_Obj_E e T l:
     Γ u⊢ₜ e : TVMem l T →
     (*─────────────────────────*)
     Γ u⊢ₜ tproj e l : T
 (** Introduction forms *)
-| Lam_typed_strong e T1 T2 Γ':
+| iT_All_I_Strong e T1 T2 Γ':
     ⊢G Γ <:* TLater <$> Γ' →
     is_unstamped_ty' (length Γ) T1 →
     (* T1 :: Γ' u⊢ₜ e : T2 → (* Would work, but allows the argument to occur in its own type. *) *)
     shift T1 :: Γ' u⊢ₜ e : T2 →
     (*─────────────────────────*)
     Γ u⊢ₜ tv (vabs e) : TAll T1 T2
-| VObj_typed ds T:
+| iT_Obj_I ds T:
     Γ |L T u⊢ds ds: T →
     is_unstamped_ty' (S (length Γ)) T →
     (*──────────────────────*)
     Γ u⊢ₜ tv (vobj ds): TMu T
 
 (** "General" rules *)
-| Var_typed x T :
+| iT_Var x T :
     (* After looking up in Γ, we must weaken T for the variables on top of x. *)
     Γ !! x = Some T →
     (*──────────────────────*)
     Γ u⊢ₜ tv (var_vl x) : shiftN x T
-| Subs_typed e T1 T2 i :
+| iT_Sub e T1 T2 i :
     Γ u⊢ₜ T1, 0 <: T2, i → Γ u⊢ₜ e : T1 →
     (*───────────────────────────────*)
     Γ u⊢ₜ iterate tskip i e : T2
-| Path_typed p T :
+| iT_Path p T :
     Γ u⊢ₚ p : T, 0 →
     (*───────────────────────────────*)
     Γ u⊢ₜ path2tm p : T
 
 (** Primitives. *)
-| T_Nat_typed n:
+| iT_Nat_I n:
     Γ u⊢ₜ tv (vnat n): TNat
-| T_Bool_typed b:
+| iT_Bool_I b:
     Γ u⊢ₜ tv (vbool b): TBool
-| T_Un_typed u e1 B1 Br (Hu : un_op_syntype u B1 Br) :
+| iT_Un u e1 B1 Br (Hu : un_op_syntype u B1 Br) :
     Γ u⊢ₜ e1 : TPrim B1 →
     Γ u⊢ₜ tun u e1 : TPrim Br
-| T_Bin_typed b e1 e2 B1 B2 Br (Hu : bin_op_syntype b B1 B2 Br) :
+| iT_Bin b e1 e2 B1 B2 Br (Hu : bin_op_syntype b B1 B2 Br) :
     Γ u⊢ₜ e1 : TPrim B1 →
     Γ u⊢ₜ e2 : TPrim B2 →
     Γ u⊢ₜ tbin b e1 e2 : TPrim Br
-| T_If_typed e e1 e2 T :
+| iT_If e e1 e2 T :
     Γ u⊢ₜ e: TBool →
     Γ u⊢ₜ e1 : T →
     Γ u⊢ₜ e2 : T →
     Γ u⊢ₜ tif e e1 e2 : T
 where "Γ u⊢ₜ e : T " := (typed Γ e T)
 with dms_typed Γ : dms → ty → Prop :=
-| dnil_typed : Γ u⊢ds [] : TTop
+| iD_Nil : Γ u⊢ds [] : TTop
 (* This demands definitions and members to be defined in aligned lists. *)
-| dcons_typed l d ds T1 T2:
+| iD_Cons l d ds T1 T2:
     Γ u⊢{ l := d } : T1 →
     Γ u⊢ds ds : T2 →
     dms_hasnt ds l →
@@ -101,173 +101,173 @@ with dms_typed Γ : dms → ty → Prop :=
     Γ u⊢ds (l, d) :: ds : TAnd T1 T2
 where "Γ u⊢ds ds : T" := (dms_typed Γ ds T)
 with dm_typed Γ : label → dm → ty → Prop :=
-| dty_typed T l L U:
+| iD_Typ_Abs T l L U:
     is_unstamped_ty' (length Γ) T →
     Γ u⊢ₜ TLater L, 0 <: TLater T, 0 →
     Γ u⊢ₜ TLater T, 0 <: TLater U, 0 →
     Γ u⊢{ l := dtysyn T } : TTMem l L U
-| dpt_pv_typed l v T:
+| iD_Val l v T:
     Γ u⊢ₜ tv v : T →
     Γ u⊢{ l := dpt (pv v) } : TVMem l T
-| dpath_typed l p T:
+| iD_Path l p T:
     Γ u⊢ₚ p : T, 0 →
     is_unstamped_path (length Γ) AlsoNonVars p →
     Γ u⊢{ l := dpt p } : TVMem l T
-| dnew_typed l T ds:
+| iD_Val_New l T ds:
     TAnd (TLater T) (TSing (pself (pv (ids 1)) l)) :: Γ u⊢ds ds : T →
     is_unstamped_ty' (S (length Γ)) T →
     Γ u⊢{ l := dpt (pv (vobj ds)) } : TVMem l (TMu T)
-| dpt_sub_typed T1 T2 p l:
+| iD_Path_Sub T1 T2 p l:
     Γ u⊢ₜ T1, 0 <: T2, 0 →
     Γ u⊢{ l := dpt p } : TVMem l T1 →
     Γ u⊢{ l := dpt p } : TVMem l T2
 where "Γ u⊢{ l := d  } : T" := (dm_typed Γ l d T)
 with path_typed Γ : path → ty → nat → Prop :=
-| pv_typed x T:
+| iP_Val x T:
     Γ u⊢ₜ tv (var_vl x) : T →
     Γ u⊢ₚ pv (var_vl x) : T, 0
 (* Mnemonic: Path from SELecting a Field *)
-| pself_typed p T i l:
+| iP_Fld_E p T i l:
     Γ u⊢ₚ p : TVMem l T, i →
     Γ u⊢ₚ pself p l : T, i
-| p_subs_typed p T1 T2 i j :
+| iP_Sub p T1 T2 i j :
     Γ u⊢ₜ T1, i <: T2, i + j →
     Γ u⊢ₚ p : T1, i →
     (*───────────────────────────────*)
     Γ u⊢ₚ p : T2, i + j
-| p_mu_i_typed p T {i} :
+| iP_Mu_I p T {i} :
     is_unstamped_ty' (S (length Γ)) T →
     Γ u⊢ₚ p : T .Tp[ p /], i →
     Γ u⊢ₚ p : TMu T, i
-| p_mu_e_typed p T {i} :
+| iP_Mu_E p T {i} :
     is_unstamped_ty' (S (length Γ)) T →
     Γ u⊢ₚ p : TMu T, i →
     Γ u⊢ₚ p : T .Tp[ p /], i
-| pself_inv_typed p T i l:
+| iP_Fld_I p T i l:
     Γ u⊢ₚ pself p l : T, i →
     (*─────────────────────────*)
     Γ u⊢ₚ p : TVMem l T, i
-| psingleton_refl_typed T p i :
+| iP_Sngl_Refl T p i :
     Γ u⊢ₚ p : T, i →
     Γ u⊢ₚ p : TSing p, i
-| psingleton_inv_typed p q i:
+| iP_Sngl_Inv p q i:
     Γ u⊢ₚ p : TSing q, i →
     is_unstamped_path' (length Γ) q →
     Γ u⊢ₚ q : TTop, i
-| psingleton_trans p q T i:
+| iP_Sngl_Trans p q T i:
     Γ u⊢ₚ p : TSing q, i →
     Γ u⊢ₚ q : T, i →
     Γ u⊢ₚ p : T, i
-| psingleton_elim T p q l i:
+| iP_Sngl_E T p q l i:
     Γ u⊢ₚ p : TSing q, i →
     Γ u⊢ₚ pself q l : T, i →
     Γ u⊢ₚ pself p l : TSing (pself q l), i
 where "Γ u⊢ₚ p : T , i" := (path_typed Γ p T i)
 (* Γ u⊢ₜ T1, i1 <: T2, i2 means that TLater^i1 T1 <: TLater^i2 T2. *)
 with subtype Γ : ty → nat → ty → nat → Prop :=
-| Refl_stp i T :
+| iSub_Refl i T :
     is_unstamped_ty' (length Γ) T →
     Γ u⊢ₜ T, i <: T, i
-| Trans_stp i2 T2 {i1 i3 T1 T3}:
+| iSub_Trans i2 T2 {i1 i3 T1 T3}:
     Γ u⊢ₜ T1, i1 <: T2, i2 →
     Γ u⊢ₜ T2, i2 <: T3, i3 →
     Γ u⊢ₜ T1, i1 <: T3, i3
-| TLaterL_stp i T:
+| iLater_Sub i T:
     is_unstamped_ty' (length Γ) T →
     Γ u⊢ₜ TLater T, i <: T, S i
-| TLaterR_stp i T:
+| iSub_Later i T:
     is_unstamped_ty' (length Γ) T →
     Γ u⊢ₜ T, S i <: TLater T, i
 
 (* "Structural" rule about indexes *)
-| TAddLater_stp T i:
+| iSub_Add_Later T i:
     is_unstamped_ty' (length Γ) T →
     Γ u⊢ₜ T, i <: TLater T, i
 
 (* "Logical" connectives *)
-| Top_stp i T :
+| iSub_Top i T :
     is_unstamped_ty' (length Γ) T →
     Γ u⊢ₜ T, i <: TTop, i
-| Bot_stp i T :
+| iBot_Sub i T :
     is_unstamped_ty' (length Γ) T →
     Γ u⊢ₜ TBot, i <: T, i
-| TAnd1_stp T1 T2 i:
+| iAnd1_Sub T1 T2 i:
     is_unstamped_ty' (length Γ) T1 →
     is_unstamped_ty' (length Γ) T2 →
     Γ u⊢ₜ TAnd T1 T2, i <: T1, i
-| TAnd2_stp T1 T2 i:
+| iAnd2_Sub T1 T2 i:
     is_unstamped_ty' (length Γ) T1 →
     is_unstamped_ty' (length Γ) T2 →
     Γ u⊢ₜ TAnd T1 T2, i <: T2, i
-| TAnd_stp T U1 U2 i j:
+| iSub_And T U1 U2 i j:
     Γ u⊢ₜ T, i <: U1, j →
     Γ u⊢ₜ T, i <: U2, j →
     Γ u⊢ₜ T, i <: TAnd U1 U2, j
-| TOr1_stp T1 T2 i:
+| iSub_Or1 T1 T2 i:
     is_unstamped_ty' (length Γ) T1 →
     is_unstamped_ty' (length Γ) T2 →
     Γ u⊢ₜ T1, i <: TOr T1 T2, i
-| TOr2_stp T1 T2 i:
+| iSub_Or2 T1 T2 i:
     is_unstamped_ty' (length Γ) T1 →
     is_unstamped_ty' (length Γ) T2 →
     Γ u⊢ₜ T2, i <: TOr T1 T2, i
-| TOr_stp T1 T2 U i j:
+| iOr_Sub T1 T2 U i j:
     Γ u⊢ₜ T1, i <: U, j →
     Γ u⊢ₜ T2, i <: U, j →
     Γ u⊢ₜ TOr T1 T2, i <: U, j
 
 (* Type selections *)
-| SelU_stp p L {l U i}:
+| iSel_Sub p L {l U i}:
     Γ u⊢ₚ p : TTMem l L U, i →
     Γ u⊢ₜ TSel p l, i <: TLater U, i
-| LSel_stp p U {l L i}:
+| iSub_Sel p U {l L i}:
     Γ u⊢ₚ p : TTMem l L U, i →
     Γ u⊢ₜ TLater L, i <: TSel p l, i
-| PSub_singleton_stp p q {i T1 T2}:
+| iSngl_pq_Sub p q {i T1 T2}:
     T1 ~Tp[ p := q ]* T2 →
     is_unstamped_ty' (length Γ) T1 →
     is_unstamped_ty' (length Γ) T2 →
     Γ u⊢ₚ p : TSing q, i →
     Γ u⊢ₜ T1, i <: T2, i
-| PSym_singleton_stp T {p q i}:
+| iSngl_Sub_Sym T {p q i}:
     Γ u⊢ₚ p : T, i →
     Γ u⊢ₜ TSing p, i <: TSing q, i →
     Γ u⊢ₜ TSing q, i <: TSing p, i
-| PSelf_singleton_stp {p T i} :
+| iSngl_Sub_Self {p T i} :
     Γ u⊢ₚ p : T, i →
     Γ u⊢ₜ TSing p, i <: T, i
 
 (* TODO: figure out if the drugs I had when I wrote these rules were good or bad. *)
-(* | SelU_stp l L U p i j: *)
+(* | iSel_Sub l L U p i j: *)
 (*     Γ u⊢ₚ p : TTMem l L U, i → *)
 (*     Γ u⊢ₜ TSel p l, j <: U, S (i + j) *)
-(* | LSel_stp l L U p i j: *)
+(* | iSub_Sel l L U p i j: *)
 (*     Γ u⊢ₚ p : TTMem l L U, i → *)
 (*     Γ u⊢ₜ L, S (i + j) <: TSel p l, j *)
 
 (* Subtyping for recursive types. Congruence, and opening in both directions. *)
-| Mu_stp_mu T1 T2 i j:
+| iMu_Sub_Mu T1 T2 i j:
     (iterate TLater i T1 :: Γ) u⊢ₜ T1, i <: T2, j →
     is_unstamped_ty' (S (length Γ)) T1 →
     Γ u⊢ₜ TMu T1, i <: TMu T2, j
-| Mu_stp T i:
+| iMu_Sub T i:
     is_unstamped_ty' (length Γ) T →
     Γ u⊢ₜ TMu (shift T), i <: T, i
-| Stp_mu T i:
+| iSub_Mu T i:
     is_unstamped_ty' (length Γ) T →
     Γ u⊢ₜ T, i <: TMu (shift T), i
 
 (* "Congruence" or "variance" rules for subtyping. Unneeded for "logical" types.
  "Cov" stands for covariance, "Con" for contravariance. *)
-| TAllConCov_stp T1 T2 U1 U2 i:
+| iAll_Sub_All T1 T2 U1 U2 i:
     Γ u⊢ₜ TLater T2, i <: TLater T1, i →
     iterate TLater (S i) (shift T2) :: Γ u⊢ₜ TLater U1, i <: TLater U2, i →
     is_unstamped_ty' (length Γ) T2 →
     Γ u⊢ₜ TAll T1 U1, i <: TAll T2 U2, i
-| TVMemCov_stp T1 T2 i l:
+| iFld_Sub_Fld T1 T2 i l:
     Γ u⊢ₜ T1, i <: T2, i →
     Γ u⊢ₜ TVMem l T1, i <: TVMem l T2, i
-| TTMemConCov_stp L1 L2 U1 U2 i l:
+| iTyp_Sub_Typ L1 L2 U1 U2 i l:
     Γ u⊢ₜ TLater L2, i <: TLater L1, i →
     Γ u⊢ₜ TLater U1, i <: TLater U2, i →
     Γ u⊢ₜ TTMem l L1 U1, i <: TTMem l L2 U2, i
@@ -276,16 +276,16 @@ with subtype Γ : ty → nat → ty → nat → Prop :=
     F[A ∧ B] <: F[A] ∧ F[B] is provable by covariance.
     Let's prove F[A] ∧ F[B] <: F[A ∧ B] in the model.
     *)
-| TAllDistr_stp T U1 U2 i:
+| iAnd_All_Sub_Distr T U1 U2 i:
     is_unstamped_ty' (length Γ) T →
     is_unstamped_ty' (S (length Γ)) U1 →
     is_unstamped_ty' (S (length Γ)) U2 →
     Γ u⊢ₜ TAnd (TAll T U1) (TAll T U2), i <: TAll T (TAnd U1 U2), i
-| TVMemDistr_stp l T1 T2 i:
+| iAnd_Fld_Sub_Distr l T1 T2 i:
     is_unstamped_ty' (length Γ) T1 →
     is_unstamped_ty' (length Γ) T2 →
     Γ u⊢ₜ TAnd (TVMem l T1) (TVMem l T2), i <: TVMem l (TAnd T1 T2), i
-| TTMemDistr_stp l L U1 U2 i:
+| iAnd_Typ_Sub_Distr l L U1 U2 i:
     is_unstamped_ty' (length Γ) L →
     is_unstamped_ty' (length Γ) U1 →
     is_unstamped_ty' (length Γ) U2 →
@@ -298,7 +298,7 @@ with subtype Γ : ty → nat → ty → nat → Prop :=
 where "Γ u⊢ₜ T1 , i1 <: T2 , i2" := (subtype Γ T1 i1 T2 i2).
 
 (* Make [T] first argument: Hide Γ for e.g. typing examples. *)
-Global Arguments dty_typed {Γ} T _ _ _ _ _ _ : assert.
+Global Arguments iD_Typ_Abs {Γ} T _ _ _ _ _ _ : assert.
 
 Scheme unstamped_typed_mut_ind := Induction for typed Sort Prop
 with   unstamped_dms_typed_mut_ind := Induction for dms_typed Sort Prop
@@ -310,8 +310,8 @@ Combined Scheme unstamped_typing_mut_ind from unstamped_typed_mut_ind, unstamped
   unstamped_path_typed_mut_ind, unstamped_subtype_mut_ind.
 
 Hint Constructors typed dms_typed dm_typed path_typed subtype : core.
-Remove Hints Trans_stp : core.
-Hint Extern 10 => try_once Trans_stp : core.
+Remove Hints iSub_Trans : core.
+Hint Extern 10 => try_once iSub_Trans : core.
 
 Lemma unstamped_path_root_is_var Γ p T i:
   Γ u⊢ₚ p : T, i → ∃ x, path_root p = var_vl x.
@@ -321,20 +321,20 @@ Lemma dtysem_not_utyped Γ l d T :
   Γ u⊢{ l := d } : T → ∀ σ s, d ≠ dtysem σ s.
 Proof. by case. Qed.
 
-Lemma Lam_typed Γ e T1 T2:
+Lemma iT_All_I Γ e T1 T2:
   is_unstamped_ty' (length Γ) T1 →
   shift T1 :: Γ u⊢ₜ e : T2 →
   (*─────────────────────────*)
   Γ u⊢ₜ tv (vabs e) : TAll T1 T2.
-Proof. apply Lam_typed_strong. ietp_weaken_ctx. Qed.
+Proof. apply iT_All_I_Strong. ietp_weaken_ctx. Qed.
 
-Lemma Lam_typed_strip1 Γ e V T1 T2:
+Lemma iT_All_I_strip1 Γ e V T1 T2:
   is_unstamped_ty' (S (length Γ)) T1 →
   shift T1 :: V :: Γ u⊢ₜ e : T2 →
   (*─────────────────────────*)
   Γ |L V u⊢ₜ tv (vabs e) : TAll T1 T2.
 Proof.
-  intros. apply Lam_typed_strong with (Γ' := (V :: Γ)) => //.
+  intros. apply iT_All_I_Strong with (Γ' := (V :: Γ)) => //.
   rewrite /defCtxCons/=; ietp_weaken_ctx.
 Qed.
 
@@ -342,28 +342,28 @@ Lemma dvabs_typed' Γ V T1 T2 e l:
   is_unstamped_ty' (S (length Γ)) T1 →
   shift T1 :: V :: Γ u⊢ₜ e : T2 →
   Γ |L V u⊢{ l := dpt (pv (vabs e)) } : TVMem l (TAll T1 T2).
-Proof. by intros; apply dpt_pv_typed, Lam_typed_strip1. Qed.
+Proof. by intros; apply iD_Val, iT_All_I_strip1. Qed.
 
 Lemma pv_dlater {Γ p T i} :
   is_unstamped_ty' (length Γ) T →
   Γ u⊢ₚ p : TLater T, i →
   Γ u⊢ₚ p : T, S i.
 Proof.
-  intros Hu Hp; apply p_subs_typed with (j := 1) (T1 := TLater T) (T2 := T) in Hp;
+  intros Hu Hp; apply iP_Sub with (j := 1) (T1 := TLater T) (T2 := T) in Hp;
     move: Hp; rewrite (plusnS i 0) (plusnO i); intros; by [|constructor].
 Qed.
 
-Ltac ettrans := eapply Trans_stp.
+Ltac ettrans := eapply iSub_Trans.
 
-(* Lemma TMono_stp {Γ T1 T2 i j} :
+(* Lemma iSub_Mono {Γ T1 T2 i j} :
   Γ u⊢ₜ T1, i <: T2, j →
   is_unstamped_ty' (length Γ) T1 →
   is_unstamped_ty' (length Γ) T2 →
   Γ u⊢ₜ T1, S i <: T2, S j.
 Proof.
   intros.
-  ettrans; first exact: TLaterR_stp.
-  ettrans; last exact: TLaterL_stp.
+  ettrans; first exact: iSub_Later.
+  ettrans; last exact: iLater_Sub.
   exact: TLater_Mono_stp.
 Qed. *)
 
@@ -373,8 +373,8 @@ Lemma Sub_later_shift {Γ T1 T2 i j}
   (Hsub: Γ u⊢ₜ T1, S i <: T2, S j):
   Γ u⊢ₜ TLater T1, i <: TLater T2, j.
 Proof.
-  ettrans; first exact: TLaterL_stp.
-  by eapply Trans_stp, TLaterR_stp.
+  ettrans; first exact: iLater_Sub.
+  by eapply iSub_Trans, iSub_Later.
 Qed.
 
 Lemma Sub_later_shift_inv {Γ T1 T2 i j}
@@ -383,13 +383,13 @@ Lemma Sub_later_shift_inv {Γ T1 T2 i j}
   (Hsub: Γ u⊢ₜ TLater T1, i <: TLater T2, j):
   Γ u⊢ₜ T1, S i <: T2, S j.
 Proof.
-  ettrans; first exact: TLaterR_stp.
-  by eapply Trans_stp, TLaterL_stp.
+  ettrans; first exact: iSub_Later.
+  by eapply iSub_Trans, iLater_Sub.
 Qed.
 
 Ltac typconstructor :=
   match goal with
-  | |- typed _ _ _ => first [apply Lam_typed_strip1 | apply Lam_typed | constructor]
+  | |- typed _ _ _ => first [apply iT_All_I_strip1 | apply iT_All_I | constructor]
   | |- dms_typed _ _ _ => constructor
   | |- dm_typed _ _ _ _ => first [apply dvabs_typed' | constructor]
   | |- path_typed _ _ _ _ => first [apply pv_dlater | constructor]
