theories/Dot/typing/typing_unstamped_derived.v
@@ -24,7 +24,7 @@ Proof. by move => /unstamped_subject_closed/fv_of_val_inv/nclosed_var_lt. Qed.
 (* Ltac tcrush := repeat first [ fast_done | typconstructor | stcrush ]. *)
 Ltac tcrush := repeat first [ eassumption | reflexivity | typconstructor | stcrush ].
 
-Lemma Appv_typed Γ e1 x2 T1 T2:
+Lemma iT_All_Ex Γ e1 x2 T1 T2:
   Γ u⊢ₜ e1: TAll T1 T2 →
   Γ u⊢ₜ tv (var_vl x2) : T1 →
   is_unstamped_ty' (S (length Γ)) T2 →
@@ -33,32 +33,32 @@ Lemma Appv_typed Γ e1 x2 T1 T2:
 Proof.
   intros He1 Hx2 Hu. have Hlx2 := var_typed_closed Hx2.
   rewrite -(psubst_subst_agree_ty (n := S (length Γ))); tcrush.
-  eapply App_path_typed with (p2 := (pv (var_vl x2))); tcrush.
+  eapply iT_All_Ex_p with (p2 := (pv (var_vl x2))); tcrush.
 Qed.
 
-Lemma TMuE_typed Γ x T:
+Lemma iT_Mu_E Γ x T:
   Γ u⊢ₜ tv (var_vl x): TMu T →
   (*──────────────────────*)
   is_unstamped_ty' (S (length Γ)) T →
   Γ u⊢ₜ tv (var_vl x): T.|[(var_vl x)/].
 Proof.
   move => + Hu. rewrite -(psubst_subst_agree_ty (n := S (length Γ))) // => Hx.
-  by apply (Path_typed (p := pv (ids x))), p_mu_e_typed, pv_typed, Hx.
+  by apply (iT_Path (p := pv (ids x))), iP_Mu_E, iP_Val, Hx.
 Qed.
 
-Lemma TMuI_typed Γ x T:
+Lemma iT_Mu_I Γ x T:
   Γ u⊢ₜ tv (var_vl x): T.|[(var_vl x)/] →
   (*──────────────────────*)
   is_unstamped_ty' (S (length Γ)) T →
   Γ u⊢ₜ tv (var_vl x): TMu T.
 Proof.
   move => + Hu. rewrite -(psubst_subst_agree_ty (n := S (length Γ))) // => Hx.
-  by apply (Path_typed (p := pv (ids x))), p_mu_i_typed, pv_typed, Hx.
+  by apply (iT_Path (p := pv (ids x))), iP_Mu_I, iP_Val, Hx.
 Qed.
 
 Ltac tcrush ::=
   repeat first [ eassumption | reflexivity |
-  apply TMuI_typed | apply TMuE_typed |
+  apply iT_Mu_I | apply iT_Mu_E |
   typconstructor | stcrush ].
 
 Lemma is_unstamped_TLater_n i {n T}:
@@ -75,11 +75,11 @@ Ltac wtcrush := repeat first [ fast_done | typconstructor | stcrush ] ; try solv
 
 Ltac asideLaters :=
   repeat first
-    [ettrans; last (apply TLaterR_stp; tcrush)|
-    ettrans; first (apply TLaterL_stp; tcrush)].
+    [ettrans; last (apply iSub_Later; tcrush)|
+    ettrans; first (apply iLater_Sub; tcrush)].
 
-Ltac lNext := ettrans; first apply TAnd2_stp; tcrush.
-Ltac lThis := ettrans; first apply TAnd1_stp; tcrush.
+Ltac lNext := ettrans; first apply iAnd2_Sub; tcrush.
+Ltac lThis := ettrans; first apply iAnd1_Sub; tcrush.
 
 Ltac lookup :=
   lazymatch goal with
@@ -108,53 +108,53 @@ Ltac hideCtx :=
   | |- ?Γ u⊢ds _ : _ => hideCtx' Γ
   end.
 
-Lemma Var_typed' Γ x T1 T2 :
+Lemma iT_Var' Γ x T1 T2 :
   Γ !! x = Some T1 →
   T2 = shiftN x T1 →
   (*──────────────────────*)
   Γ u⊢ₜ tv (var_vl x) : T2.
 Proof. intros; subst; tcrush. Qed.
 
-Lemma Var0_typed Γ T :
+Lemma iT_Var0 Γ T :
   Γ !! 0 = Some T →
   (*──────────────────────*)
   Γ u⊢ₜ tv (var_vl 0) : T.
-Proof. intros; eapply Var_typed'; by rewrite ?hsubst_id. Qed.
+Proof. intros; eapply iT_Var'; by rewrite ?hsubst_id. Qed.
 
-Ltac var := exact: Var0_typed || exact: Var_typed'.
+Ltac var := exact: iT_Var0 || exact: iT_Var'.
 
-Lemma Subs_typed_nocoerce T1 T2 {Γ e} :
+Lemma iT_Sub_nocoerce T1 T2 {Γ e} :
   Γ u⊢ₜ e : T1 →
   Γ u⊢ₜ T1, 0 <: T2, 0 →
   Γ u⊢ₜ e : T2.
 Proof. rewrite -(iterate_0 tskip e). eauto. Qed.
-Hint Resolve Subs_typed_nocoerce : core.
+Hint Resolve iT_Sub_nocoerce : core.
 
-Lemma Var_typed_sub Γ x T1 T2 :
+Lemma iT_Var_Sub Γ x T1 T2 :
   Γ !! x = Some T1 →
   Γ u⊢ₜ shiftN x T1, 0 <: T2, 0 →
   (*──────────────────────*)
   Γ u⊢ₜ tv (var_vl x) : T2.
-Proof. by intros; eapply Subs_typed_nocoerce; [var|]. Qed.
+Proof. by intros; eapply iT_Sub_nocoerce; [var|]. Qed.
 
-Lemma Var0_typed_sub Γ T1 T2 :
+Lemma iT_Var0_Sub Γ T1 T2 :
   Γ !! 0 = Some T1 →
   Γ u⊢ₜ T1, 0 <: T2, 0 →
   (*──────────────────────*)
   Γ u⊢ₜ tv (var_vl 0) : T2.
-Proof. intros. by eapply Var_typed_sub; [| rewrite ?hsubst_id]. Qed.
+Proof. intros. by eapply iT_Var_Sub; [| rewrite ?hsubst_id]. Qed.
 
-Ltac varsub := (eapply Var0_typed_sub || eapply Var_typed_sub); first done.
+Ltac varsub := (eapply iT_Var0_Sub || eapply iT_Var_Sub); first done.
 
-Lemma Appv_typed' T2 {Γ e1 x2 T1 T3} :
+Lemma iT_All_Ex' T2 {Γ e1 x2 T1 T3} :
   Γ u⊢ₜ e1: TAll T1 T2 →                        Γ u⊢ₜ tv (ids x2) : T1 →
   T3 = T2.|[ids x2/] →
   is_unstamped_ty' (S (length Γ)) T2 →
   (*────────────────────────────────────────────────────────────*)
   Γ u⊢ₜ tapp e1 (tv (ids x2)) : T3.
-Proof. intros; subst; exact: Appv_typed. Qed.
+Proof. intros; subst; exact: iT_All_Ex. Qed.
 
-Lemma TMuE_typed' Γ x T1 T2:
+Lemma iT_Mu_E' Γ x T1 T2:
   Γ u⊢ₜ tv (ids x): μ T1 →
   T2 = T1.|[ids x/] →
   is_unstamped_ty' (S (length Γ)) T1 →
@@ -162,53 +162,53 @@ Lemma TMuE_typed' Γ x T1 T2:
   Γ u⊢ₜ tv (ids x): T2.
 Proof. intros; subst; tcrush. Qed.
 
-Lemma LSel_stp' Γ U {p l L i}:
+Lemma iSub_Sel' Γ U {p l L i}:
   is_unstamped_ty' (length Γ) L →
   Γ u⊢ₚ p : TTMem l L U, i →
   Γ u⊢ₜ L, i <: TSel p l, i.
-Proof. intros; ettrans; last exact: (@LSel_stp _ p); tcrush. Qed.
+Proof. intros; ettrans; last exact: (@iSub_Sel _ p); tcrush. Qed.
 
-(** Specialization of [LSel_stp'] for convenience. *)
-Lemma LSel_stp'' Γ {p l L i}:
+(** Specialization of [iSub_Sel'] for convenience. *)
+Lemma iSub_Sel'' Γ {p l L i}:
   is_unstamped_ty' (length Γ) L →
   Γ u⊢ₚ p : TTMem l L L, i → Γ u⊢ₜ L, i <: TSel p l, i.
-Proof. apply LSel_stp'. Qed.
+Proof. apply iSub_Sel'. Qed.
 
-(* Worse than dty_typed, but shown in the paper. *)
-(* Lemma dty_typed_intermediate Γ T l L U:
+(* Worse than iD_Typ_Abs, but shown in the paper. *)
+(* Lemma iD_Typ_Abs_intermediate Γ T l L U:
   is_unstamped_ty' (length Γ) L →
   is_unstamped_ty' (length Γ) T →
   is_unstamped_ty' (length Γ) U →
   Γ u⊢ₜ L, 0 <: T, 0 →
   Γ u⊢ₜ T, 0 <: U, 0 →
   Γ u⊢{ l := dtysyn T } : TTMem l L U.
-Proof. intros; apply dty_typed => //; tcrush; exact: TMono_stp. Qed. *)
+Proof. intros; apply iD_Typ_Abs => //; tcrush; exact: iSub_Mono. Qed. *)
 
 (** * Manipulating laters, basics. *)
 
-Lemma AddIJ_stp {Γ T} i j (Hst: is_unstamped_ty' (length Γ) T) :
+Lemma iSub_AddIJ {Γ T} i j (Hst: is_unstamped_ty' (length Γ) T) :
   Γ u⊢ₜ T, j <: T, i + j.
 Proof.
   elim: i => [|n IHn]; first tcrush.
   ettrans; first apply IHn.
-  ettrans; [exact: TAddLater_stp | tcrush].
+  ettrans; [exact: iSub_Add_Later | tcrush].
 Qed.
 
-Lemma AddIJ_stp' {Γ T} i j (Hst: is_unstamped_ty' (length Γ) T) (Hle : i <= j) :
+Lemma iSub_AddIJ' {Γ T} i j (Hst: is_unstamped_ty' (length Γ) T) (Hle : i <= j) :
   Γ u⊢ₜ T, i <: T, j.
-Proof. rewrite (le_plus_minus i j Hle) Nat.add_comm. exact: AddIJ_stp. Qed.
+Proof. rewrite (le_plus_minus i j Hle) Nat.add_comm. exact: iSub_AddIJ. Qed.
 
-Lemma AddI_stp Γ T i (Hst: is_unstamped_ty' (length Γ) T) :
+Lemma iSub_AddI Γ T i (Hst: is_unstamped_ty' (length Γ) T) :
   Γ u⊢ₜ T, 0 <: T, i.
-Proof. apply (AddIJ_stp' 0 i); by [|lia]. Qed.
+Proof. apply (iSub_AddIJ' 0 i); by [|lia]. Qed.
 
 Lemma path_tp_delay {Γ p T i j} (Hst: is_unstamped_ty' (length Γ) T) : i <= j →
   Γ u⊢ₚ p : T, i → Γ u⊢ₚ p : T, j.
 Proof.
   intros Hle Hp.
   rewrite (le_plus_minus i j Hle); move: {j Hle} (j - i) => k.
-  eapply p_subs_typed, Hp.
-  apply: AddIJ_stp'; by [|lia].
+  eapply iP_Sub, Hp.
+  apply: iSub_AddIJ'; by [|lia].
 Qed.
 
 (* Lemma AddIB_stp Γ T U i:
@@ -218,17 +218,17 @@ Qed.
   Γ u⊢ₜ T, i <: U, i.
 Proof.
   move => HuT HuU Hstp; elim: i => [|n IHn]; first tcrush.
-  exact: TMono_stp.
+  exact: iSub_Mono.
 Qed. *)
 
 (** * Derived constructions. *)
 
-Lemma Let_typed Γ t u T U :
+Lemma iT_Let Γ t u T U :
   Γ u⊢ₜ t : T →
   shift T :: Γ u⊢ₜ u : shift U →
   is_unstamped_ty' (length Γ) T →
   Γ u⊢ₜ lett t u : U.
-Proof. move => Ht Hu HsT. apply /App_typed /Ht /Lam_typed /Hu /HsT. Qed.
+Proof. move => Ht Hu HsT. apply /iT_All_E /Ht /iT_All_I /Hu /HsT. Qed.
 
 Lemma val_LB L U Γ i x l :
   is_unstamped_ty' (length Γ) L →
@@ -237,7 +237,7 @@ Lemma val_LB L U Γ i x l :
   Γ u⊢ₜ tv (ids x) : type l >: L <: U →
   Γ u⊢ₜ ▶: L, i <: (pv (ids x) @; l), i.
 Proof.
-  intros ??? Hv; apply (LSel_stp (p := pv _) (U := U)).
+  intros ??? Hv; apply (iSub_Sel (p := pv _) (U := U)).
   apply (path_tp_delay (i := 0)); wtcrush.
 Qed.
 
@@ -248,7 +248,7 @@ Lemma val_UB L U Γ i x l :
   Γ u⊢ₜ tv (ids x) : type l >: L <: U →
   Γ u⊢ₜ (pv (ids x) @; l), i <: ▶: U, i.
 Proof.
-  intros ??? Hv; apply (SelU_stp (p := pv _) (L := L)).
+  intros ??? Hv; apply (iSel_Sub (p := pv _) (L := L)).
   apply (path_tp_delay (i := 0)); wtcrush.
 Qed.
 
@@ -265,7 +265,7 @@ Proof. intros; apply /val_LB /packTV_typed'. Qed. *)
   Γ u⊢ₜ (pv (packTV T) @; "A"), i <: ▶: T, i.
 Proof. intros; by apply /val_UB /packTV_typed'. Qed. *)
 
-Lemma Dty_typed Γ T l:
+Lemma iD_Typ Γ T l:
   is_unstamped_ty' (length Γ) T →
   Γ u⊢{ l := dtysyn T } : TTMem l T T.
 Proof. intros. tcrush. Qed.
@@ -278,8 +278,8 @@ Lemma Bind1 Γ T1 T2 i:
   Γ u⊢ₜ μ T1, i <: T2, i.
 Proof.
   intros Hus1 Hus2 Hsub.
-  ettrans; first exact: (Mu_stp_mu Hsub).
-  exact: Mu_stp.
+  ettrans; first exact: (iMu_Sub_Mu Hsub).
+  exact: iMu_Sub.
 Qed.
 
 Lemma Bind2 Γ T1 T2 i:
@@ -288,7 +288,7 @@ Lemma Bind2 Γ T1 T2 i:
   Γ u⊢ₜ T1, i <: μ T2, i.
 Proof.
   intros Hus1 Hus2 Hsub.
-  ettrans; last apply (Mu_stp_mu Hsub); [exact: Stp_mu | wtcrush].
+  ettrans; last apply (iMu_Sub_Mu Hsub); [exact: iSub_Mu | wtcrush].
 Qed.
 
 Lemma Bind1' Γ T1 T2:
@@ -314,63 +314,63 @@ Lemma BindSpec Γ (L T U : ty):
   Γ u⊢ₜ tv (ν {@ type "A" = T }) : μ {@ type "A" >: L <: U }.
 Proof.
   intros.
-  eapply Subs_typed_nocoerce with (T1 := μ {@ type "A" >: T <: T }); ltcrush.
+  eapply iT_Sub_nocoerce with (T1 := μ {@ type "A" >: T <: T }); ltcrush.
 Qed.
 
-Lemma p_subs_typed' {Γ p T1 T2 i} :
+Lemma iP_Sub' {Γ p T1 T2 i} :
   Γ u⊢ₜ T1, i <: T2, i →
   Γ u⊢ₚ p : T1, i →
   (*───────────────────────────────*)
   Γ u⊢ₚ p : T2, i.
 Proof.
   intros; rewrite -(plusnO i).
-  by eapply p_subs_typed; rewrite ?plusnO.
+  by eapply iP_Sub; rewrite ?plusnO.
 Qed.
 
-Lemma psingleton_sym_typed Γ p q i:
+Lemma iP_Sngl_Sym Γ p q i:
   is_unstamped_path' (length Γ) q →
   Γ u⊢ₚ p : TSing q, i →
   Γ u⊢ₚ q : TSing p, i.
 Proof.
-  intros Hus Hpq. eapply p_subs_typed'.
-  eapply (PSym_singleton_stp Hpq). by apply PSelf_singleton_stp, Hpq.
-  eapply psingleton_refl_typed.
-  by apply (psingleton_inv_typed Hpq).
+  intros Hus Hpq. eapply iP_Sub'.
+  eapply (iSngl_Sub_Sym Hpq). by apply iSngl_Sub_Self, Hpq.
+  eapply iP_Sngl_Refl.
+  by apply (iP_Sngl_Inv Hpq).
 Qed.
 
-Lemma PSub_singleton_stp_inv {Γ i p q T1 T2}:
+Lemma iSngl_pq_Sub_inv {Γ i p q T1 T2}:
   T1 ~Tp[ p := q ]* T2 →
   is_unstamped_ty' (length Γ) T1 →
   is_unstamped_ty' (length Γ) T2 →
   is_unstamped_path' (length Γ) p →
   Γ u⊢ₚ q : TSing p, i →
   Γ u⊢ₜ T1, i <: T2, i.
-Proof. intros. by eapply PSub_singleton_stp, psingleton_sym_typed. Qed.
+Proof. intros. by eapply iSngl_pq_Sub, iP_Sngl_Sym. Qed.
 
-Lemma pand_typed {Γ p T1 T2 i}:
+Lemma iP_And {Γ p T1 T2 i}:
   Γ u⊢ₚ p : T1, i →
   Γ u⊢ₚ p : T2, i →
   Γ u⊢ₚ p : TAnd T1 T2, i.
 Proof.
-  intros Hp1 Hp2. eapply p_subs_typed', psingleton_refl_typed, Hp1.
-  constructor; exact: PSelf_singleton_stp.
+  intros Hp1 Hp2. eapply iP_Sub', iP_Sngl_Refl, Hp1.
+  constructor; exact: iSngl_Sub_Self.
 Qed.
 
-Lemma Mu_stp' {Γ T T' i}:
+Lemma iMu_Sub' {Γ T T' i}:
   T' = shift T →
   is_unstamped_ty' (length Γ) T →
   Γ u⊢ₜ μ T', i <: T, i.
 Proof. intros; subst. auto. Qed.
 
-Lemma dvabs_sub_typed {Γ} V T1 T2 e l L:
+Lemma iD_Lam_Sub {Γ} V T1 T2 e l L:
   shift T1 :: V :: Γ u⊢ₜ e : T2 →
   TLater V :: Γ u⊢ₜ TAll T1 T2, 0 <: L, 0 →
   is_unstamped_ty' (S (length Γ)) T1 →
   Γ |L V u⊢{ l := dpt (pv (vabs e)) } : TVMem l L.
 Proof.
-  intros He Hsub Hs. apply dpt_pv_typed.
-  eapply (Subs_typed (i := 0)); first apply Hsub.
-  by apply Lam_typed_strip1.
+  intros He Hsub Hs. apply iD_Val.
+  eapply (iT_Sub (i := 0)); first apply Hsub.
+  by apply iT_All_I_strip1.
 Qed.
 
 (* Note how we must weaken the type (or its environment) to account for the
@@ -383,9 +383,9 @@ Lemma packTV_typed' T n Γ l :
   Γ u⊢ₜ tv (packTV l T) : typeEq l T.
 Proof.
   move => HsT1 Hle; move: (Hle) (HsT1) => /le_n_S Hles /is_unstamped_ren1_ty HsT2.
-  apply (Subs_typed_nocoerce (μ {@ typeEq l (shift T) }));
-    last (ettrans; first apply: (Mu_stp _ (T := {@ typeEq l T })); wtcrush).
-  apply VObj_typed; wtcrush.
+  apply (iT_Sub_nocoerce (μ {@ typeEq l (shift T) }));
+    last (ettrans; first apply: (iMu_Sub _ (T := {@ typeEq l T })); wtcrush).
+  apply iT_Obj_I; wtcrush.
 Qed.
 
 Lemma packTV_typed T Γ l :
@@ -407,13 +407,13 @@ Lemma tyApp_typed Γ T U V t l :
   Γ u⊢ₜ tyApp t l T : V.
 Proof.
   move => Ht Hsub HuT1 HuU1.
-  eapply Let_typed; [exact: Ht| |wtcrush].
-  eapply Let_typed; [apply packTV_typed| |]; wtcrush.
+  eapply iT_Let; [exact: Ht| |wtcrush].
+  eapply iT_Let; [apply packTV_typed| |]; wtcrush.
   rewrite /= -!hrenS -/(typeEq _ _).
 
-  apply /Subs_typed_nocoerce /Hsub.
+  apply /iT_Sub_nocoerce /Hsub.
 
-  eapply Appv_typed'; first var.
+  eapply iT_All_Ex'; first var.
   have HuT3 : is_unstamped_ty' (S (S (length Γ))) (shiftN 2 T)
     by rewrite hrenS; wtcrush.
   varsub; tcrush; rewrite !hsubst_comp; f_equal. autosubst.
@@ -425,24 +425,24 @@ Qed.
 (** * Manipulating laters, more.
 
  *)
-Lemma TLaterRN_stp Γ T i j:
+Lemma iSub_LaterN Γ T i j:
   is_unstamped_ty' (length Γ) T →
   Γ u⊢ₜ T, j + i <: iterate TLater j T, i.
 Proof.
   elim: j T => /= [|j IHj] T HuT; rewrite ?iterate_0 ?iterate_Sr /=; tcrush.
   ettrans.
-  - exact: TLaterR_stp.
+  - exact: iSub_Later.
   - apply (IHj (TLater T)); stcrush.
 Qed.
 
-Lemma TLaterLN_stp {Γ T} i j :
+Lemma iLaterN_Sub {Γ T} i j :
   is_unstamped_ty' (length Γ) T →
   Γ u⊢ₜ iterate TLater j T, i <: T, j + i.
 Proof.
   elim: j T => /= [|j IHj] T HuT; rewrite ?iterate_0 ?iterate_Sr /=; tcrush.
   ettrans.
   - apply (IHj (TLater T)); stcrush.
-  - exact: TLaterL_stp.
+  - exact: iLater_Sub.
 Qed.
 
 (* This can be useful when [T] is a singleton type. *)
@@ -454,10 +454,10 @@ Lemma dropLaters Γ e T U i:
   Γ u⊢ₜ iterate tskip i e : TAnd T U.
 Proof.
   intros HeT Hsub HuT HuU.
-  eapply Subs_typed, HeT => {HeT}.
-  typconstructor; [exact: AddI_stp|] => {HuT}.
+  eapply iT_Sub, HeT => {HeT}.
+  typconstructor; [exact: iSub_AddI|] => {HuT}.
   ettrans; [apply: Hsub|] => {Hsub}.
-  have := (TLaterLN_stp 0 i HuU); rewrite plusnO; exact.
+  have := (iLaterN_Sub 0 i HuU); rewrite plusnO; exact.
 Qed.
 
 (**
@@ -475,8 +475,8 @@ Lemma deLaterSingV0 {Γ} p i e T U:
   Γ u⊢ₜ deLater (path2tm p) i e : U.
 Proof.
   intros HpT1 Hsub HeU HuT Hup.
-  apply Let_typed with (T := TSing p); tcrush.
-  apply Let_typed with (T := TAnd (shift (TSing p)) T); rewrite /= -?hrenS; wtcrush.
+  apply iT_Let with (T := TSing p); tcrush.
+  apply iT_Let with (T := TAnd (shift (TSing p)) T); rewrite /= -?hrenS; wtcrush.
   apply dropLaters; [ var | .. ]; rewrite /= -?hrenS; wtcrush.
 Qed.
 
@@ -492,9 +492,9 @@ Lemma deLaterSingV1 {Γ} p i e T1 T2 U:
   Γ u⊢ₜ deLater (path2tm p) i e : U.
 Proof.
   intros HpT1 Hsub HeU HuT1 HuT2 Hup.
-  apply Let_typed with (T := TAnd (TSing p) T1); tcrush.
-  by apply pand_typed, HpT1; eapply psingleton_refl_typed, HpT1.
-  apply Let_typed with (T := TAnd (shift (TAnd (TSing p) T1)) T2); rewrite /= -?hrenS; wtcrush.
+  apply iT_Let with (T := TAnd (TSing p) T1); tcrush.
+  by apply iP_And, HpT1; eapply iP_Sngl_Refl, HpT1.
+  apply iT_Let with (T := TAnd (shift (TAnd (TSing p) T1)) T2); rewrite /= -?hrenS; wtcrush.
   apply dropLaters; [ var | lNext | ..]; rewrite /= -?hrenS; wtcrush.
 Qed.
 
@@ -508,60 +508,60 @@ Lemma deLaterSing {Γ} p i e T1 U:
   Γ u⊢ₜ deLater (path2tm p) i e : U.
 Proof.
   intros HpT1 HeU HuT1 Hup.
-  apply Let_typed with (T := TAnd (TSing p) (iterate TLater i T1)); wtcrush.
-  by apply pand_typed, HpT1; eapply psingleton_refl_typed, HpT1.
-  apply Let_typed with (T := TAnd (TSing (shift p)) (shift T1));
+  apply iT_Let with (T := TAnd (TSing p) (iterate TLater i T1)); wtcrush.
+  by apply iP_And, HpT1; eapply iP_Sngl_Refl, HpT1.
+  apply iT_Let with (T := TAnd (TSing (shift p)) (shift T1));
     rewrite /= -?hrenS ?TLater_subst; wtcrush.
-  eapply Subs_typed; last var; tcrush; [lThis|lNext]; wtcrush.
-  by apply: AddI_stp; wtcrush.
-  rewrite -{3}(plusnO i). apply TLaterLN_stp; wtcrush.
+  eapply iT_Sub; last var; tcrush; [lThis|lNext]; wtcrush.
+  by apply: iSub_AddI; wtcrush.
+  rewrite -{3}(plusnO i). apply iLaterN_Sub; wtcrush.
 Qed.
 
 Lemma selfIntersect Γ T U i j:
   is_unstamped_ty' (length Γ) T →
   Γ u⊢ₜ T, i <: U, j + i →
   Γ u⊢ₜ T, i <: TAnd U T, j + i .
-Proof. intros; tcrush. exact: AddIJ_stp. Qed.
+Proof. intros; tcrush. exact: iSub_AddIJ. Qed.
 
-Lemma TDistr_TLater_And_stp Γ T1 T2 i :
+Lemma iAnd_Later_Sub_Distr Γ T1 T2 i :
   is_unstamped_ty' (length Γ) T1 →
   is_unstamped_ty' (length Γ) T2 →
   Γ u⊢ₜ TAnd (TLater T1) (TLater T2), i <: TLater (TAnd T1 T2), i.
 Proof. intros; asideLaters; tcrush; [lThis|lNext]. Qed.
 
-(** Inverse of [TDistr_TLater_And_stp]. *)
-Lemma TDistr_TLater_And_stp_inv Γ T1 T2 i :
+(** Inverse of [iAnd_Later_Sub_Distr]. *)
+Lemma iAnd_Later_Sub_Distr_inv Γ T1 T2 i :
   is_unstamped_ty' (length Γ) T1 →
   is_unstamped_ty' (length Γ) T2 →
   Γ u⊢ₜ TLater (TAnd T1 T2), i <: TAnd (TLater T1) (TLater T2), i.
 Proof. intros; tcrush. Qed.
 
-Lemma TDistr_TLater_Or_stp Γ T1 T2 i :
-  is_unstamped_ty' (length Γ) T1 →
-  is_unstamped_ty' (length Γ) T2 →
-  Γ u⊢ₜ TLater (TOr T1 T2), i <: TOr (TLater T1) (TLater T2), i.
-Proof.
-  intros; asideLaters; typconstructor; ettrans;
-    [| apply TOr1_stp | | apply TOr2_stp]; tcrush.
-Qed.
-
-(** Inverse of [TDistr_TLater_Or_stp]. *)
-Lemma TDistr_TLater_Or_stp_inv Γ T1 T2 i :
+Lemma iOr_Later_Sub_Distr Γ T1 T2 i :
   is_unstamped_ty' (length Γ) T1 →
   is_unstamped_ty' (length Γ) T2 →
   Γ u⊢ₜ TOr (TLater T1) (TLater T2), i <: TLater (TOr T1 T2), i.
 Proof. intros; tcrush. Qed.
 
+(** Inverse of [iOr_Later_Sub_Distr]. *)
+Lemma iOr_Later_Sub_Distr_inv Γ T1 T2 i :
+  is_unstamped_ty' (length Γ) T1 →
+  is_unstamped_ty' (length Γ) T2 →
+  Γ u⊢ₜ TLater (TOr T1 T2), i <: TOr (TLater T1) (TLater T2), i.
+Proof.
+  intros; asideLaters; typconstructor; ettrans;
+    [| apply iSub_Or1 | | apply iSub_Or2]; tcrush.
+Qed.
+
 (** TLater swaps with TMu, part 1. *)
-Lemma TDistr_TLater_Mu_stp Γ T i :
+Lemma iMu_Later_Sub_Distr Γ T i :
   is_unstamped_ty' (S (length Γ)) T →
-  Γ u⊢ₜ TLater (TMu T), i <: TMu (TLater T), i.
+  Γ u⊢ₜ TMu (TLater T), i <: TLater (TMu T), i.
 Proof. intros; asideLaters; tcrush. Qed.
 
 (** TLater swaps with TMu, part 2. *)
-Lemma TDistr_TLater_Mu_stp_inv Γ T i :
+Lemma iMu_Later_Sub_Distr_inv Γ T i :
   is_unstamped_ty' (S (length Γ)) T →
-  Γ u⊢ₜ TMu (TLater T), i <: TLater (TMu T), i.
+  Γ u⊢ₜ TLater (TMu T), i <: TMu (TLater T), i.
 Proof. intros; asideLaters; tcrush. Qed.
 
 (** Show that [singleton_Mu_[12]] and [p_mu_[ie]_typed] are interderivable. *)
@@ -569,30 +569,30 @@ Lemma singleton_Mu_1 {Γ p T i} :
   Γ u⊢ₚ p : TMu T, i →
   is_unstamped_ty' (S (length Γ)) T →
   Γ u⊢ₜ TSing p, i <: T .Tp[ p /], i.
-Proof. intros Hp Hu; apply PSelf_singleton_stp, (p_mu_e_typed Hu Hp). Qed.
+Proof. intros Hp Hu; apply iSngl_Sub_Self, (iP_Mu_E Hu Hp). Qed.
 
 Lemma singleton_Mu_2 {Γ p T i} :
   Γ u⊢ₚ p : T .Tp[ p /], i →
   is_unstamped_ty' (S (length Γ)) T →
   Γ u⊢ₜ TSing p, i <: TMu T, i.
-Proof. intros Hp Hu; apply PSelf_singleton_stp, (p_mu_i_typed Hu Hp). Qed.
+Proof. intros Hp Hu; apply iSngl_Sub_Self, (iP_Mu_I Hu Hp). Qed.
 
-(* Avoid automation, to ensure we don't use [p_mu_e_typed] to show them. *)
-Lemma p_mu_e_typed' {Γ T p i} :
+(* Avoid automation, to ensure we don't use [iP_Mu_E] to show them. *)
+Lemma iP_Mu_E' {Γ T p i} :
   Γ u⊢ₚ p : TMu T, i →
   is_unstamped_ty' (S (length Γ)) T →
   Γ u⊢ₚ p : T .Tp[ p /], i.
 Proof.
-  intros Hp Hu. eapply p_subs_typed', (psingleton_refl_typed Hp).
+  intros Hp Hu. eapply iP_Sub', (iP_Sngl_Refl Hp).
   apply (singleton_Mu_1 Hp Hu).
 Qed.
 
-Lemma p_mu_i_typed' {Γ T p i} :
+Lemma iP_Mu_I' {Γ T p i} :
   Γ u⊢ₚ p : T .Tp[ p /], i →
   is_unstamped_ty' (S (length Γ)) T →
   Γ u⊢ₚ p : TMu T, i.
 Proof.
-  intros Hp Hu. eapply p_subs_typed', (psingleton_refl_typed Hp).
+  intros Hp Hu. eapply iP_Sub', (iP_Sngl_Refl Hp).
   apply (singleton_Mu_2 Hp Hu).
 Qed.
 
@@ -601,7 +601,7 @@ Show soundness of subtyping for recursive types in the Dotty compiler — just c
 
 The first case is in
 https://github.com/lampepfl/dotty/blob/0.20.0-RC1/compiler/src/dotty/tools/dotc/core/TypeComparer.scala#L550-L552
-And that matches Mu_stp_mu.
+And that matches iMu_Sub_Mu.
 
 https://github.com/lampepfl/dotty/blob/0.20.0-RC1/compiler/src/dotty/tools/dotc/core/TypeComparer.scala#L554-L557
 We formalize that as the derived rule below.
@@ -620,7 +620,7 @@ Lemma singleton_Mu_dotty1 {Γ p i T1' T2} :
 Proof.
   intros Hsub Hp Hu.
   apply singleton_Mu_2, Hu.
-  apply (p_subs_typed' Hsub Hp).
+  apply (iP_Sub' Hsub Hp).
 Qed.
 
 Definition anfBind t := lett t (tv x0).
@@ -630,13 +630,13 @@ Lemma AnfBind_typed Γ t (T U: ty) :
   shift T :: Γ u⊢ₜ tv x0 : shift U →
   is_unstamped_ty' (length Γ) T →
   Γ u⊢ₜ anfBind t : U.
-Proof. intros; eapply Let_typed; eauto. Qed.
+Proof. intros; eapply iT_Let; eauto. Qed.
 
 Lemma pDOT_Def_Path_derived Γ l p T
   (Hx : Γ u⊢ₚ p : T, 0)
   (Hu : is_unstamped_path (length Γ) AlsoNonVars p) :
   Γ u⊢{ l := dpt p } : TVMem l (TSing p).
-Proof. eapply dpath_typed, Hu. apply (psingleton_refl_typed (T := T)), Hx. Qed.
+Proof. eapply iD_Path, Hu. apply (iP_Sngl_Refl (T := T)), Hx. Qed.
 
 (*
 Lemma dpath_sub_typed_admit_failed Γ l p T1 T2:
@@ -645,7 +645,7 @@ Lemma dpath_sub_typed_admit_failed Γ l p T1 T2:
   Γ u⊢{ l := dpt p } : TVMem l T2.
 Proof.
   intros Ht1 Hsub; inverse Ht1; constructor => //; first
-    [eapply (Subs_typed (i := 0)) | eapply (p_subs_typed (i := 0))]; eauto.
-  apply VObj_typed; tcrush.
+    [eapply (iT_Sub (i := 0)) | eapply (iP_Sub (i := 0))]; eauto.
+  apply iT_Obj_I; tcrush.
 Abort.
 *)
