correspondence.md
@@ -36,7 +36,7 @@ Translation table:
 For each rule, there are up to three versions, with corresponding prefixes.
 - Purely semantic lemma (s)
 - Syntactic lemma
-- Syntactic typing rule (?, they still don't follow this naming convention :-( ).
+- Syntactic typing rule (i for inductive, but most still don't follow this naming convention :-().
 
 ## Differences between our paper (and technical appendix) and our Coq development.
 
